coq-minuska/theories/symex.v
@@ -5,20 +5,112 @@ From Minuska Require Import
     properties
     minusl_syntax
     unification_interface
-    symex_spec
+    (* symex_spec *)
     valuation_merge
 .
 
+Locate imap.
+Check imap.
 
-Require Import Wellfounded.
-From stdpp Require Import lexico well_founded.
 
-Require Import Program.
-From Coq Require Import Logic.Eqdep_dec.
+Equations? decouple
+    {Σ : StaticModel}
+    (et : TermOver Expression2)
+    (avoid : gset variable)
+    :
+    ((TermOver BuiltinOrVar)*(listset (variable * Expression2 )))%type
+    by wf (TermOver_size et) lt
+:=
+    decouple (t_over e) avoid :=
+        let y : variable := fresh (avoid) in
+        (t_over (bov_variable y), singleton (y,e))
+    ;
+    decouple (t_term s l) avoid :=
+        let l'' := imap (fun (i : nat) (x : TermOver Expression2) =>
+            let avoidi := avoid ∪ (union_list (vars_of <$> (take i l))) in
+            let pi_sigmai := decouple x avoidi in
+            pi_sigmai
+        ) l in
+    (t_term s (fmap fst l''), union_list (fmap snd l''))
+.
+Proof.
+    Search sum_list
+Qed.
 
-From Equations Require Export Equations.
 
-Module Implementation.
+Fixpoint decouple
+    {Σ : StaticModel}
+    (et : TermOver Expression2)
+    (avoid : gset variable)
+    :
+    ((TermOver BuiltinOrVar)*(listset (variable * Expression2 )))%type
+:=
+match et with
+| t_over e =>
+    let y : variable := fresh (avoid) in
+    (t_over (bov_variable y), singleton (y,e))
+| t_term s l =>
+    let l'' := imap (fun (i : nat) (x : TermOver Expression2) =>
+        let avoidi := avoid ∪ (union_list (vars_of <$> (take i l))) in
+        let pi_sigmai := decouple x avoidi in
+        pi_sigmai
+    ) l in
+    (* let l'' := (fix go
+        (l' : list (TermOver Expression2))
+        (avoid' : gset variable)
+        : list ((TermOver BuiltinOrVar)*(listset (variable * Expression2 )))
+        :=
+        match l' with
+        | [] => []
+        | x::xs => 
+            let pi := decouple x (avoid' ∪ (vars_of x)) in
+            pi::(go xs (avoid' ∪ (vars_of x)))
+        end
+    ) l avoid in *)
+    (t_term s (fmap fst l''), union_list (fmap snd l''))
+end
+.
 
-End Implementation.
+Lemma decouple_avoids
+    {Σ : StaticModel}
+    (et : TermOver Expression2)
+    (avoid : gset variable)
+    :
+    (vars_of (decouple et avoid).1) ## avoid
+.
+Proof.
+    revert avoid.
+    induction et;
+        intros avoid;
+        simpl in *;
+        unfold vars_of;
+        simpl.
+    {
+        unfold vars_of; simpl.
+        rewrite disjoint_singleton_l.
+        rewrite <- elem_of_elements.
+        apply infinite_is_fresh.
+    }
+    {
+        revert avoid H.
+        induction l; intros avoid H; simpl in *.
+        {
+            apply disjoint_empty_l.
+        }
+        {
+            rewrite disjoint_union_l.
+            rewrite Forall_cons in H.
+            destruct H as [Hx Hxs].
+            specialize (IHl avoid Hxs).
+            clear Hxs.
+            split.
+            {
+                simpl.
+                apply Hx.
+            }
+            {
 
+            }
+        }
+    }
+Qed.
